src/imm/CombRelationsMore.v
@@ -1,4 +1,4 @@
-From hahn Require Import Hahn.
+(* From hahn Require Import Hahn.
 From PromisingLib Require Import Loc.
 Require Import Events.
 Require Import Execution.
@@ -429,4 +429,4 @@ Qed.
 
 End CombRelationsMore.
 
-End CombRelationsMore.
+End CombRelationsMore. *)
