src/imm/HbFsupp.v
@@ -1,4 +1,4 @@
-Require Import Classical Peano_dec Setoid PeanoNat.
+(* Require Import Classical Peano_dec Setoid PeanoNat.
 From hahn Require Import Hahn.
 From hahnExt Require Import HahnExt.
 Require Import Lia.
@@ -132,4 +132,4 @@ Section HbFsupp.
   
 End HbFsupp. 
 
-End HbFsupp.
+End HbFsupp. *)
